
\section{The complex field}

\mybox{
    rudin 引入复数定义的方法很奇怪, 
    使用复数的代数定义直接引入(天上掉下来的定义).
    理解起来比较困难.

    我觉得使用几何方法引入复数更为合理且直观, 
    rudin 这里对初学者不太友好.
}

\begin{myDef}
    \label{myDef:1.24}
    A complex number is an ordered pair $(a, b)$ of real numbers.
    "Ordered" means that $(a, b)$ and $(b, a)$ are regarded as distinct if $a \neq b$.

    Let$x = (a, b)$, $y = (c,d)$ be two complex numbers. 
    We write $x =y$ if and only if $a =c$ and $b=d$. 
    (Note that this definition is not entirely superfluous;
    think of equality of rational numbers, 
    represented as quotients of integers.) 
    We define
    \begin{align*}
        x+y &= (a + c, b + d),\\
        xy  &= (ac - bd, ad + bc).
    \end{align*}
\end{myDef}

\begin{thm}
    \label{thm:1.25}
    These definitions of addition and multiplication 
    turn the \emph{set} of all complex numbers into a field, 
    with $(0, 0)$ and $(1, 0)$ in the role $0$ and $1$.
\end{thm}

\mybox{
    proof (A1)--(A5), (M1)--(M5) and (D), 

    then we can prove that $\mathbb{C}$ is a field.
}

\begin{thm}
    \label{thm:1.26}
    For any real numbers $a$ and $b$ we have
    \begin{equation*}
        (a,0)+ (b,0) = (a+ b,0),\quad
        (a,0)(b,0) = (ab,0).
    \end{equation*}
\end{thm}
The proof is trivial.

show that the notation $(a, b)$ is equivalent to the more customary $a + bi$.

\begin{myDef}
    \label{myDef:1.27}
    $i=(0,1)$    
\end{myDef}

\begin{thm}
    \label{thm:1.28}
    $i^2=-1$
\end{thm}

\begin{proof}
    \begin{equation*}
        i^2=(0,1)(0,1)=(-1,0)=-1.
    \end{equation*}
\end{proof}

\begin{thm}
    \label{thm:1.29}
    If $a$ and $b$ are real, then $(a,b) =a + bi$.
\end{thm}

\begin{proof}
    \begin{align*}
        a+bi
        &=(a,0)+(b,0)(0,1)\\
        &=(a,0)+(0,b)=(a,b)\\
    \end{align*}
\end{proof}

\begin{myDef}
    \label{myDef:1.30}
    $a,b\in \R$, $z = a + bi$,
    the complex number $\bar{z} = a  -bi$ is called the conjugate of $z$.
    the numbers $a$ and $b$ are the real part and imaginary part of $z$.
    respectively.
    \begin{equation*}
        a=\Re(z), \quad
        b=\Im(z)
    \end{equation*}
\end{myDef}

\begin{thm}
    \label{thm:1.31}
    If $z$ and $w$ are complex, then
    \begin{enumerate}[(a)]
        \item $\bar{z+w}=\bar{z}+\bar{w}$,
        \item $\bar{zw}=\bar{z}\cdot\bar{w}$,
        \item $z+\bar{z}=2\Re(z)$, $z-\bar{z}=2\Im(z)$,
        \item $z\bar{z}$ is real and positive (except when $z=0$).
    \end{enumerate}
\end{thm}

\myproof{
    (a), (b),and (c)are quite trivial.
    To prove (d), write $z = a + bi$,
    and note that $z\bar{z} = a^2 + b^2$.
}

\begin{myDef}
    \label{myDef:1.32}
    If $z$ is a complex number, 
    its absolute value $|z|$ is the nonnegative square root of $z\bar{z}$; 
    that is, $|z| = (z\bar{z})^{1/2}$.
\end{myDef}
The existence (and uniqueness) of $|z|$ follows from Theorem \ref{thm:1.21} and part (d) of Theorem \ref{thm:1.31}.

Note that when $x$ is real, then $\bar{x} = x$, 
hence $|x| = \sqrt{x^2}$. Thus $|x| = x$
if $x>0$, $|x| = -x$ if $x <0$.

\begin{thm}
    \label{thm:1.33}
    Let $z$ and $w$ be complex numbers. Then
    \begin{enumerate}[(a)]
        \item $|z|>0$ unless $z=0$, $|0|=0$,
        \item $\bar{z}=z$,
        \item $|zw| = |z||w|$,
        \item $| \Re(z)| \leq |z|$,
        \item $|z+w| \leq|z|+|w|$.
    \end{enumerate}
\end{thm}


\begin{myNotation}(Big sum)
    \label{myNotation:1.34}
    $x_1,x_2,\dots,x_n \in \mathbb{C}$,
    \begin{equation*}
        x_1+x_2+\dots+x_n = \sum_{j=1}^{n} x_j.
    \end{equation*}
\end{myNotation}

\begin{thm}(Schwarz Inequality)
    \label{thm:1.35}
    If 
    $a_1,\dots,a_n$, 
    $b_1,\dots,b_n$, are complex numbers, then
    \begin{equation*}
        \left| \sum_{j=1}^{n}a_j \bar{b_j}\right|^2 \leq 
        \sum_{j=1}^{n}\left|a_j\right|^2
        \sum_{j=1}^{n}\left|b_j\right|^2.
    \end{equation*}    
\end{thm}

\myproof{
    在正式证明之前, 先回忆 $\R$ 中的施瓦茨不等式是怎么证明的.
    let $A = \sum a_j^2$, $B = \sum b_j^2$, $C = \sum a_j b_j$.
    \begin{equation*}
        \sum (a_j+\lambda b_j)^2 = 
        \sum a_j^2 
        + 2\sum a_j b_j \lambda
        + \sum b_j^2 \lambda^2
    \end{equation*}
    由韦达定理, $\Delta \leq 0$, 
    $\Delta= (2\sum a_j b_j )^2 - 4 \sum a_j^2\sum b_j^2$. 
    因此 $(\sum a_j b_j )^2 \leq \sum a_j^2\sum b_j^2$.
}

\begin{proof}
    Put $A = \sum |a_j|^2$, $B = \sum |b_j|^2$, $C = \sum a_j \bar{b_j}$, $j = 1,2,\dots,n$. \\    
    If $B = 0$, $b_1 = \dots = b_n = 0$, this conclusion is trivial.\\
    If $B > 0$, 
    \begin{align*}
        \sum \left|B a_j - C b_j\right|^2
        &= \sum (B a_j-C b_j)(B \bar{a_j} - \bar{C b_j})\\
        &= B^2\sum \left|a_j\right|^2 - B\bar{C}\sum a_j \bar{b_j} - BC \sum \bar{a_j} b_j + \left|C\right|^2\sum |b_j|^2\\
        &= B^2A-B|C|^2\\
        &= B(AB-|C|^2).
    \end{align*}
    Since each term in the first sum is nonnegative, we see that
    \begin{equation*}
        B(AB-|C|^2) \geq 0.
    \end{equation*}
    Since $B>0$, it follows that $AB-|C|^2 \geq 0$. This is the desired inequality.
\end{proof}

\myproof{
    我的想法
    \begin{align*}
        \sum (a_j + \lambda \bar{b_j})(\bar{a_j} + \lambda b_j)
        &=\sum(
            a_j\bar{a_j}
            + \lambda(\bar{a_j}b_j+a_j\bar{b_j})
            + \lambda^2 b_j\bar{b_j}
            )\\
        &= A + \lambda (C + \bar{C}) + \lambda^{2} B
    \end{align*}
    由韦达定理, $\Delta \leq 0$, 
    % $\Delta = (\sum\Re(a_j\bar{b_j}))^2-4\sum a_j\bar{a_j}\sum b_j\bar{b_j}$, 
    $\Delta = (C + \bar{C})^2-4AB \leq 0$, 
    (这里推出的结论比原始结论弱？为什么？)

    $A = \sum \left| a_j \right|^2 $,
    $B = \sum \left| b_j \right|^2 $,
    $C = \sum a_j \bar{b}_j$.
    \begin{align*}
        \left| C \right|^2 
        &= C \cdot \bar{C}\\
        &= \left( \sum a_j \bar{b}_j \right) 
        \overline{\left( \sum a_j \bar{b}_j \right)}.\\
        &= \left( \sum a_j \bar{b}_j \right) 
        \left( \sum \overline{a_j \bar{b}_j} \right).\\
        &= \left( \sum a_j \bar{b}_j \right) 
        \left( \sum \bar{a}_j {b}_j \right).
    \end{align*}

    可不可以用 $C^2 + \bar{C}^2 \geq 2 C \bar{C}$?
    
}