# 题目
$$
    C_{100}^0 \biggl(\frac{1}{2}\biggr)^{100}
    +C_{99}^1 \biggl(\frac{1}{2}\biggr)^{99}
    +\dots
    +C_{51}^{49} \biggl(\frac{1}{2}\biggr)^{100}
    +C_{50}^{50} \biggl(\frac{1}{2}\biggr)^{100}
$$
对上式求和 
[来源](https://www.zhihu.com/question/402309978/answer/2582880019)

## 解答
[来源](https://www.zhihu.com/question/402309978/answer/2582880019)

置
$$
    A_n:=\sum_{i=0}^{n}\binom{n+i}{n-i}\frac{1}{2^{n+i}}
    =\sum_{i=0}^{n}\binom{n+i}{2i}\frac{1}{2^{n+i}},
$$

所求即为 $A_{50}$ . 为了求出 $A_n$ 的通项，考虑利用**生成函数**，设 $f(x)=\sum_{n=0}^{\infty}A_n x^n$ ， 则有
$$
    \begin{align*}
        f(x) 
        &= \sum_{n=0}^{\infty}A_n x^n \\
        &= \sum_{n=0}^{\infty} \Biggl[\sum_{i=0}^{\infty}\binom{n+i}{2i}\frac{1}{2^{n+i}}\Biggr] x^n \\
        &= \sum_{i=0}^{\infty} \frac{1}{2^i} \sum_{n=i}^{\infty}\binom{n+i}{2i}\biggl(\frac{x}{2}\biggr)^{n} \text{  交换求和次序}\\
        &= \sum_{i=0}^{\infty} \frac{1}{2^i} \sum_{n=0}^{\infty}\binom{n+2i}{2i}\biggl(\frac{x}{2}\biggr)^{n+i} \text{  换元 } n\rightarrow n+i \\
        &= \sum_{i=0}^{\infty} \frac{x^i}{4^i} \sum_{n=0}^{\infty}\binom{n+2i}{2i}\biggl(\frac{x}{2}\biggr)^{n} \\
        &= \sum_{i=0}^{\infty} \frac{x^i}{4^i}\frac{1}{(1-\frac{x}{2})^{2i+1}} \\
        &= \frac{1}{(1-\frac{x}{2})}\sum_{i=0}^{\infty} \biggl(\frac{x}{4(1-\frac{x}{2})^2}\biggr)^i \\
        &= \frac{2}{2-x}\sum_{i=0}^{\infty} \biggl(\frac{x}{(2-x)^2}\biggr)^i \\
        &= \frac{2}{2-x}\cdot \frac{1}{1-\frac{x}{(2-x)^2}} \\
        &= \frac{2(2-x)}{(2-x)^2-x} \\
        &= \frac{2(2-x)}{4-5x+x^2} \\
        &= \frac{2(2-x)}{(x-4)(x-1)} \\
        &= \frac{-4}{3(x-4)} + \frac{-2}{3(x-1)} \\
        &= \frac{4}{3(4-x)} + \frac{2}{3(1-x)} \\
        &= \frac{1}{3}\sum_{n=0}^{\infty}\biggl(\frac{x}{4}\biggr)^n + \frac{2}{3}\sum_{n=0}^{\infty}x^n\\
        &= \sum_{n=0}^{\infty}\biggl(
            \frac{2}{3}+
            \frac{1}{3\cdot 4^n}
        \biggr)x^n,\\
    \end{align*}
$$

所以 $A_n=\frac{2}{3}+\frac{1}{3\cdot 4^n}$ , 赋值 $n=50$ 代入即可。